\section*{Problem 2}

Convert the following \(n\)-th order linear differential equation (\( y^{(j)} \) denotes the \(j\)-th derivative)
\[
    y^{(n)}(t) + a_{n-1}(t) y^{(n-1)}(t) + a_{n-2}(t) y^{(n-2)}(t) + \cdots + a_{1}(t) y^{(1)}(t) + a_{0}(t) y(t) = b_0(t) u(t) + b_1(t) u^{(1)}(t)
\]
into the following type of equation:
\begin{align*}
    \dot{x}(t) & = A(t) x(t) + B(t) u(t) \\
    y(t)       & = C(t) x(t) + D(t) u(t)
\end{align*}

\textit{Hint:} Let, \( x^{(n)}(t) = y^{(n-1)}(t) - b_1(t)u(t) \)

\subsection*{Solution}
