\section*{Problem 4}

Consider the system
\begin{equation*}
    \dot{x}_{1}=x_{2}, \quad \dot{x}_{2}=2 x_{1} x_{2}+3 t+2-3 x_{1}-2(t+1) x_{2}
\end{equation*}
\begin{enumerate}[label= (\alph*)]
    \item Verify that, \( x(t)=[t, 1]^{\top} \) is a solution of the system.
    \item Show that if \( x(0) \) is sufficiently close to \( [0,1]^{\top} \), then \( x(t) \) approaches \( [t, 1]^{\top} \) as \( t \rightarrow \infty \).
\end{enumerate}

\subsection*{Solution}

\subsubsection*{(a) Verification of solution \( x(t) = {[t, 1]}^\top \)}

Given the system
\begin{align*}
    \dot{x}_{1}
     & =
    x_2
    \\
    \dot{x}_{2}
     & =
    2 x_{1} x_{2} + 3 t + 2 - 3 x_{1} - 2(t + 1) x_{2}
\end{align*}
We can see that \( x(t) = {[t, 1]}^\top \) is a solution of the system by substituting the values of \( x_1 \) and \( x_2 \) in the above system, thereby we have
\begin{align*}
    \implies
    \dot{x}_{1}
     & =
    \frac{d}{dt} t
    =
    1
    =
    x_2
    \\
    \implies
    2 x_{1} x_{2} + 3 t + 2 - 3 x_{1} - 2(t + 1) x_{2}
     & =
    2 t \cdot 1 + 3 t + 2 - 3 t - 2(t + 1) \cdot 1
    \\ & =
    2 t + 3 t + 2 - 3 t - 2 t - 2
    \\ & =
    0
    =
    \frac{d}{dt} 1
    =
    \dot{x}_{2}
\end{align*}
Thus, we have verified that \( x(t) = {[t, 1]}^\top \) is indeed a solution of the system.

\subsubsection*{(b) Asymptotic stability of \( x(t) = {[t, 1]}^\top \)}

We will apply a change of variables to the given system using \( z(t) = x(t) - {[t, 1]}^\top \), thereby we have
\begin{align*}
    \dot{z}_{1}
     & =
    \dot{x}_{1} - \frac{d}{dt} t
    =
    x_2 - 1
    =
    z_2
    \\
    \dot{z}_{2}
     & =
    \dot{x}_{2} - \frac{d}{dt} 1
    =
    2 x_{1} x_{2} + 3 t + 2 - 3 x_{1} - 2(t + 1) x_{2} - 0
    \\ & =
    2 x_{1} x_{2} + 3 t + 2 - 3 x_{1} - 2(t + 1) x_{2}
    \\ & =
    2 (z_1 + t) (z_2 + 1) + 3 t + 2 - 3 (z_1 + t) - 2(t + 1) (z_2 + 1)
    \\ & =
    2 z_1 z_2 + 2 z_1 + \cancel{2 t z_2} + \cancel{2 t} + \cancel{3 t} + \cancel{2} - 3 z_1 - \cancel{3 t} - \cancel{2 t z_2} - \cancel{2 t} - 2 z_2 - \cancel{2}
    \\ & =
    2 z_1 z_2 - z_1 - 2 z_2
\end{align*}
We can see that the original problem is equivalent to showing that the origin is asymptotically stable for the new system.
We will first linearize the system around the origin, thereby we have the Jacobian matrix as
\begin{equation*}
    J
    =
    \begin{bmatrix}
        \frac{\partial \dot{z}_{1}}{\partial z_1} & \frac{\partial \dot{z}_{1}}{\partial z_2} \\
        \frac{\partial \dot{z}_{2}}{\partial z_1} & \frac{\partial \dot{z}_{2}}{\partial z_2}
    \end{bmatrix}
    =
    \begin{bmatrix}
        0         & 1         \\
        2 z_2 - 1 & 2 z_1 - 2
    \end{bmatrix}
    \implies
    A = J|_{z=0}
    =
    \begin{bmatrix}
        0  & 1  \\
        -1 & -2
    \end{bmatrix}
    \implies
    \dot{z} = A z
\end{equation*}
The characteristic equation of the matrix \( A \) is given by
\begin{align*}
    \det(A - \lambda I)
     & =
    \det
    \begin{bmatrix}
        -\lambda & 1            \\
        -1       & -2 - \lambda
    \end{bmatrix}
    =
    \lambda^2 + 2 \lambda + 1
    =
    {(\lambda + 1)}^2
    \implies
    \lambda = \{ -1, -1 \}
\end{align*}
Since all the eigenvalues of the matrix \( A \) have negative real parts, we can conclude that the origin is asymptotically stable for the system.
Thereby, we have that if \( x(0) \) is sufficiently close to \( {[0, 1]}^\top \), then \( x(t) \) approaches \( {[t, 1]}^\top \) as \( t \rightarrow \infty \).
