\section*{Problem 4}

Determine the State Transition Matrix \( \Phi(t,t_0) \) for the following system:
\begin{equation*}
    \dot x(t)
    =
    e^{-A} B e^A x(t)
\end{equation*}
Further, what will be the change in STM if A and B commute?

\subsection*{Solution}

Given the homogeneous linear time-invariant system:
\begin{equation*}
    \dot{x}(t) = e^{-A} B e^A x(t),
    \quad
    x(t_0) = x_0
\end{equation*}
We have the state transition matrix given by
\begin{align*}
    \Phi(t, t_0)
     & =
    e^{e^{-A} B e^A} x_0
    \\
    \implies
    e^{e^{-A} B e^A}
    & =
    I + e^{-A} B e^A + \frac{1}{2!} {(e^{-A} B e^A)}^2 + \frac{1}{3!} {(e^{-A} B e^A)}^3 + \ldots
    \\ & =
    \sum_{k=0}^{\infty} \frac{1}{k!} {(e^{-A} B e^A)}^k
\end{align*}
We can see that
\begin{align*}
    {(e^{-A} B e^A)}^k
     & =
     (e^{-A} B e^A)
     (e^{-A} B e^A)
     \cdots
     (e^{-A} B e^A)
    \\ & =
    e^{-A} B (e^A
    e^{-A}) B (e^A
    \cdots
    e^{-A}) B e^A
    \\ & =
    e^{-A} B^k e^{-A}
\end{align*}
\begin{align*}
    \implies
    \Phi(t, t_0)
    & =
    \sum_{k=0}^{\infty} \frac{1}{k!} {(e^{-A} B e^A)}^k
    \\ & =
    \sum_{k=0}^{\infty} \frac{1}{k!} e^{-A} B^k e^{-A}
    \\ & =
    e^{-A} \left( \sum_{k=0}^{\infty} \frac{1}{k!} B^k \right) e^{-A}
    \\ & =
    e^{-A} e^{B} e^{-A}
\end{align*}
\begin{equation*}
    \implies
    \boxed{
        \Phi(t, t_0)
        =
        e^{-A} e^{B} e^{-A} \; x(t_0)
    }
\end{equation*}
