\section*{Problem 1}

Consider a system is modeled by the following differential equation:
\[
    \ddot y - 2t\dot y - (2 - t^2)y = 0
\]
\begin{enumerate}[label= (\alph*)]
    \item Show that the following are two equivalent state-space representations of the above system:
          \begin{align*}
              \dot x
               & =
              \begin{bmatrix}
                  0       & 1  \\
                  2 - t^2 & 2t
              \end{bmatrix}
              x
              :=
              A_1(t) x
              \\
              \dot z
               & =
              \begin{bmatrix}
                  t & 1 \\
                  1 & t
              \end{bmatrix}
              z
              :=
              A_2(t) z
          \end{align*}
          \textit{Hint:} \(x\) and \(z\) share a common component.
    \item Using the easiest choice, compute the state transition matrix \(\Phi(t, 0)\)
    \item Find \(P(t)\) such that \( z(t) = P(t)x(t) \).
          What property should \(P(t)\) satisfy to be a meaningful transformation matrix?
          Is it holding in this case?
    \item Let, \( \dot{x}(t)=A(t) x+B(t) u \) be a LTV system, and \( z(t)=P(t) x(t) \) is a transformation with \( P(t) \geq 0, \forall t \geq t_{0} \).
          Derive the LTV system that describes the dynamics of \( z \).
    \item Verify your relations in part (d) using \( A_{1}(t), A_{2}(t), P(t) \) of the above example.
\end{enumerate}

\subsection*{Solution}

\subsubsection*{(a) Two equivalent state-space representations}

Given the differential equation \( \ddot y - 2t\dot y - (2 - t^2)y = 0 \),
let \( x = \begin{bmatrix} x_1 \\ x_2 \end{bmatrix} = \begin{bmatrix} y \\ \dot y \end{bmatrix} \).
Then, we have
\begin{align*}
    \implies
    \dot x_1
     & =
    \dot y = x_2
    \\
    \implies
    \dot x_2
     & =
    \ddot y = 2t\dot y + (2 - t^2)y = 2tx_2 + (2 - t^2)x_1
\end{align*}
Therefore, the state-space representation of the system is given by
\begin{align*}
    \begin{bmatrix}
        \dot x_1 \\
        \dot x_2
    \end{bmatrix}
     & =
    \begin{bmatrix}
        0       & 1  \\
        2 - t^2 & 2t
    \end{bmatrix}
    \begin{bmatrix}
        x_1 \\
        x_2
    \end{bmatrix}
    \implies
    \dot x
    =
    \begin{bmatrix}
        0       & 1  \\
        2 - t^2 & 2t
    \end{bmatrix}
    x
    :=
    A_1(t) x
\end{align*}

Now, consider \( z = \begin{bmatrix} z_1 \\ z_2 \end{bmatrix} = \begin{bmatrix} y \\ -t y + \dot y \end{bmatrix} \).
(Note: it is easier to determine this by solving part (c) first).
Then, we have
\begin{align*}
    \implies
    \dot z_1
     & =
    \dot y = z_2 + t y
    =
    z_2 + t z_1
    \\
    \implies
    \dot z_2
     & =
    \frac{d}{dt} (-t y + \dot y)
    =
    (-t \dot y - y) + \ddot y
    \\ & =
    (-t \dot y - y) + \left( 2t \dot y + (2 - t^2)y \right)
    \\ & =
    t \dot y + y - t^2 y
    \\ & =
    t (z_2 + t z_1) + z_1 - t^2 z_1
    \\ & =
    t z_2 + \cancel{t^2 z_1} + z_1 - \cancel{t^2 z_1}
    \\ & =
    t z_2 + z_1
\end{align*}
Thereby, the state-space representation of the system is equivalently given by
\begin{align*}
    \begin{bmatrix}
        \dot z_1 \\
        \dot z_2
    \end{bmatrix}
     & =
    \begin{bmatrix}
        t & 1 \\
        1 & t
    \end{bmatrix}
    \begin{bmatrix}
        z_1 \\
        z_2
    \end{bmatrix}
    \implies
    \dot z
    =
    \begin{bmatrix}
        t & 1 \\
        1 & t
    \end{bmatrix}
    z
    :=
    A_2(t) z
\end{align*}

\subsubsection*{(b) State transition matrix}

For the system \( \dot z = A_2(t) z \), we can compute the state transition matrix, by first defining \( M(t) \) as
\begin{equation*}
    M(t)
    =
    \int_{0}^{t} A_2(\tau) d\tau
    =
    \int_{0}^{t} \begin{bmatrix}
        \tau & 1    \\
        1    & \tau
    \end{bmatrix}
    d\tau
    =
    \begin{bmatrix}
        \int_{0}^{t} \tau d\tau & \int_{0}^{t} d\tau      \\
        \int_{0}^{t} d\tau      & \int_{0}^{t} \tau d\tau
    \end{bmatrix}
    =
    \begin{bmatrix}
        \frac{t^2}{2} & t             \\
        t             & \frac{t^2}{2}
    \end{bmatrix}
\end{equation*}
Checking for the commutativity of \( M(t) \) and \( A_2(t) \) as follows,
\begin{align*}
    A_2(t) M(t)
     & =
    \begin{bmatrix}
        t & 1 \\
        1 & t
    \end{bmatrix}
    \begin{bmatrix}
        \frac{t^2}{2} & t             \\
        t             & \frac{t^2}{2}
    \end{bmatrix}
    =
    \begin{bmatrix}
        \frac{t^3}{2} + t & \frac{3t^2}{2}    \\
        \frac{3t^2}{2}    & \frac{t^3}{2} + t
    \end{bmatrix}
    \\
    M(t) A_2(t)
     & =
    \begin{bmatrix}
        \frac{t^2}{2} & t             \\
        t             & \frac{t^2}{2}
    \end{bmatrix}
    \begin{bmatrix}
        t & 1 \\
        1 & t
    \end{bmatrix}
    =
    \begin{bmatrix}
        \frac{t^3}{2} + t & \frac{3t^2}{2}    \\
        \frac{3t^2}{2}    & \frac{t^3}{2} + t
    \end{bmatrix}
\end{align*}
Thereby, \( M(t) \) and \( A_2(t) \) commute, and the state transition matrix is given by
\begin{equation*}
    \Phi(t, 0)
    =
    e^{M(t)}
    =
    I + M(t) + \frac{1}{2!} {(M(t))}^2 + \frac{1}{3!} {(M(t))}^3 + \ldots
    =
    \sum_{k=0}^{\infty} \frac{1}{k!} {(M(t))}^k
\end{equation*}
We can diagonalise \( M(t) \) as follows.
The eigenvalues can be found by solving the characteristic equation \( \text{det}(M(t) - \lambda I) = 0 \), as
\begin{align*}
    \text{det}(M(t) - \lambda I)
     & =
    \text{det}\left(
    \begin{bmatrix}
            \frac{t^2}{2} - \lambda & t                       \\
            t                       & \frac{t^2}{2} - \lambda
        \end{bmatrix}
    \right)
    =
    \left( \frac{t^2}{2} - \lambda \right)^2 - t^2
    \\ & =
    \lambda^2 - t^2 \lambda + \left(\frac{t^4}{4} - t^2\right)
    =
    0
    \implies
    \lambda
    =
    \frac{t^2}{2} \pm t
\end{align*}
The eigenvectors corresponding to the eigenvalues \( \frac{t^2}{2} + t \) and \( \frac{t^2}{2} - t \) can be calculated to be \( \begin{bmatrix} 1 \\ 1 \end{bmatrix} \) and \( \begin{bmatrix} 1 \\ -1 \end{bmatrix} \) respectively, giving
\begin{equation*}
    P = \begin{bmatrix}
        1 & 1  \\
        1 & -1
    \end{bmatrix}
    \implies
    P^{-1} = \frac{1}{2} \begin{bmatrix}
        1 & 1  \\
        1 & -1
    \end{bmatrix}
\end{equation*}
Thereby, the matrix \( M(t) \) can be diagonalised as
\begin{equation*}
    M(t)
    =
    PDP^{-1}
    =
    P
    \begin{bmatrix}
        \frac{t^2}{2} + t & 0                 \\
        0                 & \frac{t^2}{2} - t
    \end{bmatrix}
    P^{-1}
\end{equation*}
From this, we can compute \( e^{M(t)} \) as
\begin{align*}
    e^{M(t)}
     & =
    \sum_{k=0}^{\infty} \frac{1}{k!} {(M(t))}^k
    =
    \sum_{k=0}^{\infty} \frac{1}{k!} P D^k P^{-1}
    =
    P \left( \sum_{k=0}^{\infty} \frac{1}{k!} D^k \right) P^{-1}
    =
    P e^D P^{-1}
    \\
     & =
    \begin{bmatrix}
        1 & 1  \\
        1 & -1
    \end{bmatrix}
    \begin{bmatrix}
        e^{\frac{t^2}{2} + t} & 0                     \\
        0                     & e^{\frac{t^2}{2} - t}
    \end{bmatrix}
    \frac{1}{2}
    \begin{bmatrix}
        1 & 1  \\
        1 & -1
    \end{bmatrix}
    \\
     & =
    \frac{1}{2}
    \begin{bmatrix}
        e^{\frac{t^2}{2} + t} + e^{\frac{t^2}{2} - t} & e^{\frac{t^2}{2} + t} - e^{\frac{t^2}{2} - t} \\
        e^{\frac{t^2}{2} + t} - e^{\frac{t^2}{2} - t} & e^{\frac{t^2}{2} + t} + e^{\frac{t^2}{2} - t}
    \end{bmatrix}
    =
    \frac{1}{2} e^{\frac{t^2}{2}}
    \begin{bmatrix}
        (e^t + e^{-t}) & (e^t - e^{-t}) \\
        (e^t - e^{-t}) & (e^t + e^{-t})
    \end{bmatrix}
    \\
     & =
    e^{\frac{t^2}{2}}
    \begin{bmatrix}
        \cosh t & \sinh t \\
        \sinh t & \cosh t
    \end{bmatrix}
\end{align*}
Thereby, the state transition is given by
\begin{equation*}
    \boxed{
        \Phi(t, 0)
        =
        e^{\frac{t^2}{2}}
        \begin{bmatrix}
            \cosh t & \sinh t \\
            \sinh t & \cosh t
        \end{bmatrix}
    }
\end{equation*}

\subsubsection*{(c) Transformation matrix \( P(t) \)}

Given the transformation matrix given by \( z(t) = P(t)x(t) \), and the expressions for \( x(t) \) and \( z(t) \) from section (a), we have
\begin{align*}
    \begin{bmatrix}
        z_1 \\
        z_2
    \end{bmatrix}
     & =
    \begin{bmatrix}
        p_{11} & p_{12} \\
        p_{21} & p_{22}
    \end{bmatrix}
    \begin{bmatrix}
        x_1 \\
        x_2
    \end{bmatrix}
    =
    \begin{bmatrix}
        p_{11} x_1 + p_{12} x_2 \\
        p_{21} x_1 + p_{22} x_2
    \end{bmatrix}
    =
    \begin{bmatrix}
        p_{11} y + p_{12} \dot y \\
        p_{21} y + p_{22} \dot y
    \end{bmatrix}
    \\
    \implies
    z_1
     & =
    y
    =
    p_{11} y + p_{12} \dot y
    \implies
    p_{11} = 1, \quad p_{12} = 0
    \\
    \implies
    z_2
     & =
    -t y + \dot y
    =
    p_{21} y + p_{22} \dot y
    \implies
    p_{21} = -t, \quad p_{22} = 1
\end{align*}
Thereby, we get the transformation matrix as
\begin{equation*}
    \boxed{
        P(t)
        =
        \begin{bmatrix}
            1  & 0 \\
            -t & 1
        \end{bmatrix}
    }
\end{equation*}
Such similarity transformations are meaningful if \( P(t) \) is differentiable and invertible and doesn't alter the system characteristics, i.e., \( \dot P(t) \) exists and \( P(t) \) is non-singular.
In this case, \( P(t) \) is differentiable and invertible, and hence, the transformation is meaningful.

\subsubsection*{(d) LTV system for \( z \)}

Given the LTV system \( \dot{x}(t)=A(t) x+B(t) u \) and the transformation \( z(t)=P(t) x(t) \), with \( P(t) \geq 0, \forall t \geq t_{0} \), we have
\begin{align*}
    \dot{z}(t)
     & =
    \frac{d}{dt} z(t)
    =
    \frac{d}{dt} (P(t) x(t))
    =
    \frac{d}{dt} \Big(P(t)\Big) x(t) + P(t) \frac{d}{dt} x(t)
    \\
     & =
    \dot{P}(t) x(t) + P(t) \Big( A(t) x(t) + B(t) u(t) \Big)
    \\ & =
    \Big( \dot{P}(t) + P(t) A(t) \Big) x(t) + P(t) B(t) u(t)
\end{align*}

For an invertible matrix \( P(t) \), we can write \( x(t) = P^{-1}(t) z(t) \), thereby giving the LTV system for \( z \) as
\[
    \boxed{
        \begin{aligned}
            \dot{z}(t)
             & =
            \tilde{A}(t) z(t) + \tilde{B}(t) u(t), \quad \text{where}
            \\
            \tilde{A}(t)
             & =
            \dot{P}(t) P^{-1}(t) + P(t) A(t) P^{-1}(t)
            \\
            \tilde{B}(t)
             & =
            P(t) B(t)
        \end{aligned}
    }
\]

\subsubsection*{(e) Verification}

For the given system, we have
\[
    A_1(t) =
    \begin{bmatrix}
        0       & 1  \\
        2 - t^2 & 2t
    \end{bmatrix}, \quad
    A_2(t) =
    \begin{bmatrix}
        t & 1 \\
        1 & t
    \end{bmatrix}, \quad
    P(t) =
    \begin{bmatrix}
        1  & 0 \\
        -t & 1
    \end{bmatrix}
\]
\begin{align*}
    \implies
    \dot{P}(t)
     & =
    \begin{bmatrix}
        0  & 0 \\
        -1 & 0
    \end{bmatrix}
    , \quad
    P^{-1}(t)
    =
    \begin{bmatrix}
        1 & 0 \\
        t & 1
    \end{bmatrix}
    \\
    \implies
    \tilde{A}(t)
     & =
    \begin{bmatrix}
        0  & 0 \\
        -1 & 0
    \end{bmatrix}
    \begin{bmatrix}
        1 & 0 \\
        t & 1
    \end{bmatrix}
    +
    \begin{bmatrix}
        1  & 0 \\
        -t & 1
    \end{bmatrix}
    \begin{bmatrix}
        0       & 1  \\
        2 - t^2 & 2t
    \end{bmatrix}
    \begin{bmatrix}
        1 & 0 \\
        t & 1
    \end{bmatrix}
    \\ & =
    \begin{bmatrix}
        0  & 0 \\
        -1 & 0
    \end{bmatrix}
    +
    \begin{bmatrix}
        1  & 0 \\
        -t & 1
    \end{bmatrix}
    \begin{bmatrix}
        t                & 1  \\
        (2 - t^2 + 2t^2) & 2t
    \end{bmatrix}
    \\ & =
    \begin{bmatrix}
        0  & 0 \\
        -1 & 0
    \end{bmatrix}
    +
    \begin{bmatrix}
        t                                                  & 1        \\
        (-\cancel{t^2} + 2 - \cancel{t^2} + \cancel{2t^2}) & (2t - t)
    \end{bmatrix}
    \\ & =
    \begin{bmatrix}
        0  & 0 \\
        -1 & 0
    \end{bmatrix}
    +
    \begin{bmatrix}
        t & 1 \\
        2 & t
    \end{bmatrix}
    =
    \begin{bmatrix}
        t & 1 \\
        1 & t
    \end{bmatrix}
    =
    A_2(t)
\end{align*}
as required.
Hence, it stands verified.
