\section*{Problem 2}

Consider the system:
\begin{equation*}
    \begin{gathered}
        \dot{x}_{1}=-x_{1}+a x_{2}-b x_{1} x_{2}+x_{2}^{2} \\
        \dot{x}_{2}=-(a+b) x_{1}+b x_{1}^{2}-x_{1} x_{2}
    \end{gathered}
\end{equation*}
where \( a>0, b \neq 0 \).

\begin{enumerate}[label= (\alph*)]
    \item Find all the equilibrium points of the system.
    \item Determine the type of each equilibrium point for all values of \( a>0, b \neq 0 \).
    \item Construct the phase portrait for the following cases and discuss the qualitative behavior of the system:
          \begin{enumerate}[label= (\roman*)]
              \item \( \mathrm{a}=\mathrm{b}=1 \)
              \item \( \mathrm{a}=1, \mathrm{~b}=-\frac{1}{2} \)
          \end{enumerate}
\end{enumerate}

\subsection*{Solution}

\subsubsection*{(a) Equilibrium Points}

The equilibrium points are obtained by setting state derivatives to zero.
Starting with the second equation, we get
\begin{align*}
    \implies
    \dot x_2
     & =
    0
    =
    -(a + b) x_1 + b x_1^2 - x_1 x_2
    =
    x_1 \left( b x_1 - x_2 - (a + b) \right)
    =
    0
    \\
    \implies
    x_1
     & =
    0
    \quad \text{or} \quad
    b x_1 - x_2 - (a + b)
    =
    0
\end{align*}
Putting \( x_1 = 0 \) in the first equation, we get
\begin{align*}
    \implies
    \dot x_1
     & =
    0
    =
    -x_1 + a x_2 - b x_1 x_2 + x_2^2
    =
    a x_2 + x_2^2
    =
    x_2 \left( a + x_2 \right)
    =
    0
    \\
    \implies
    x_2
     & =
    0
    \quad \text{or} \quad
    a + x_2
    =
    0
\end{align*}
For the other equilibrium points, we can see that
\begin{align*}
    b x_1 - x_2 - (a + b)
     & =
    0
    \\
    \implies
    x_2
     & =
    b x_1 - (a + b)
\end{align*}
Substituting this in the first equation, we get
\begin{align*}
    \implies
    \dot x_1
     & =
    0
    =
    -x_1 + a \left( b x_1 - (a + b) \right) - b x_1 \left( b x_1 - (a + b) \right) + \left( b x_1 - (a + b) \right)^2
    \\
    \implies
    0
     & =
    -x_1 + a b x_1 - a (a + b) - b x_1 \left( b x_1 - (a + b) \right) + \left( b x_1 - (a + b) \right)^2
    \\
    \implies
    0
     & =
    -x_1 + a b x_1 - a (a + b) - \cancel{b^2 x_1^2} + b (a + b) x_1 + \cancel{b^2 x_1^2} - 2 b (a + b) x_1 + (a + b)^2
    \\
    \implies
    0
     & =
    -x_1 + a b x_1 - b (a + b) x_1 + b(a + b)
\end{align*}
\begin{align*}
    \implies
    0
     & =
    x_1 \left( -1 + a b - b (a + b) \right) + b(a + b)
    \\
    \implies
    0
     & =
    x_1 \left( -1 + \cancel{a b} - \cancel{b a} - b^2 \right) + b(a + b)
    \\
    \implies
    x_1
     & =
    \frac{b(a + b)}{b^2 + 1}
\end{align*}
Putting this back in the equation for \( x_2 \), we get
\begin{align*}
    x_2
     & =
    b x_1 - (a + b)
    =
    b \left( \frac{b(a + b)}{b^2 + 1} \right) - (a + b)
    \\ & =
    \frac{b^2(a + b) - (a + b)(b^2 + 1)}{b^2 + 1}
    =
    \frac{\cancel{b^2 a} + \cancel{b^3} - \cancel{a b^2} - a - \cancel{b^3} - b}{b^2 + 1}
    \\
    \implies
    x_1
     & =
    \frac{-(a+b)}{b^2 + 1}
\end{align*}

Thereby, the equilibrium points are
\begin{equation*}
    \boxed{
        x^* =
        \left \{ \;
        \begin{bmatrix}
            0 \\
            0
        \end{bmatrix}, \; \;
        \begin{bmatrix}
            0 \\
            -a
        \end{bmatrix}, \; \;
        \frac{a+b}{b^2 + 1}
        \begin{bmatrix}
            -1 \\
            b
        \end{bmatrix} \;
        \right \}
    }
\end{equation*}
